reorganize files

theories/Firstorder.v
@@ -6,159 +6,12 @@ From MetaCoq.PCUIC Require Import PCUICAst PCUICTyping PCUICFirstorder PCUICCase
 From MetaCoq.Erasure Require Import EWcbvEval EWcbvEvalNamed.
 From MetaCoq.SafeChecker Require Import PCUICErrors PCUICWfEnv PCUICWfEnvImpl.
 
-From Malfunction Require Import Malfunction SemanticsSpec utils_array Compile.
+From Malfunction Require Import Malfunction SemanticsSpec utils_array Compile RealizabilitySemantics.
 
 Require Import ZArith Array.PArray List String Floats Lia Bool.
 Import ListNotations.
 From MetaCoq.Utils Require Import bytestring.
 
-Print nat_rect.
-
-Unset Elimination Schemes. 
-
-Inductive camlType : Set :=
-    Arrow : camlType -> camlType -> camlType
-  | Rel : nat -> camlType
-  | Adt : kername -> 
-            (* number of the ADT in the mutual definition *) nat -> 
-            (* list of parameters *) list camlType -> 
-            camlType.
-
-Definition camlType_rect :
-forall P : camlType -> Type,
-       (forall c : camlType,
-        P c -> forall c0 : camlType, P c0 -> P (Arrow c c0)) ->
-       (forall n : nat, P (Rel n)) ->
-       (forall (k : kername) i (l : list camlType), All P l -> P (Adt k i l)) ->
-       forall c : camlType, P c. 
-Proof. 
-  intros P X X0 X1. fix f 1. intros c; destruct c.
-  - eapply X; eauto.   
-  - eapply X0; eauto. 
-  - eapply X1; eauto. induction l; econstructor; eauto. 
-Defined.
-       
-Set Elimination Schemes. 
-
-Notation "A → B" := (Arrow A B) (at level 50). 
-
-Definition isArrow T := match T with Arrow _ _ => true | _ => false end.
-
-Definition ADT : Set := 
-  (* number of parameters *)
-  nat * list (
-    list (list camlType) (* list of constructors for each ADT *)).
-
-Inductive Existsi {A : Type} (P : nat -> A -> Prop) (n : nat) 
-  : list A -> Prop :=
-	  Existsi_cons_hd : forall x l, P n x -> Existsi P n (x :: l)
-  | Existsi_cons_tl : forall (x : A) (l : list A),
-                     Existsi P (S n) l -> Existsi P n (x :: l).
-
-Lemma Existsi_spec A (P : nat -> A -> Prop) n (l:list A) : Existsi P n l -> 
-  exists k x, n <= k /\ k < n + List.length l /\ P k x /\ nth_error l (k-n) = Some x.
-Proof.
-  induction 1.
-  - exists n; exists x. cbn; repeat split; eauto. lia.
-    now rewrite Nat.sub_diag.   
-  - destruct IHExistsi as [k [a [Hk [Hk' [HP Ha]]]]].
-    exists k; exists a. repeat split; eauto; cbn; try lia.
-    assert (k - n = S (k - S n)) by lia.
-    now rewrite H0. 
-Defined. 
-
-Section Realizability. 
-
-  Variable _Heap:Heap.
-
-  Definition realize_adt_type := 
-      forall (params: list camlType), All (fun _ => value -> Prop) params -> 
-              ((* number of the ADT in the mutual definition *) nat -> value -> Prop).
-
-  Variable globals : list (Ident.t * value).
-  
-  Definition global_adt_decl := list (kername * realize_adt_type).
-
-  Open Scope bs. 
-
-  Definition empty_locals : Ident.Map.t := fun _ => fail "not_defined".
-
-  Close Scope bs. 
-
-  Section Values. 
-
-    Variable local_adt : list (value -> Prop).
-    Variable global_adt : global_adt_decl.
-
-    Definition to_realize_term (realize_val : value -> Prop) 
-      : t -> Prop := fun t => forall h h' v, 
-      eval _ globals empty_locals h t h' v -> realize_val v.
-
-    Definition to_realize_value (realize_term : t -> Prop) 
-      : value -> Prop := fun v => exists t h h', 
-        eval _ globals empty_locals h t h' v /\ realize_term t.
-
-    Definition realize_term (A:camlType) : t -> Prop.
-    Proof.
-      refine (camlType_rect _ _ _ _ A); clear A.
-      - intros A PA B PB.
-        exact (fun f => forall t, PA t -> PB (Mapply(f,[t]))).
-      - intros n. 
-        exact (to_realize_term (List.nth n local_adt (fun _ => False))).
-      - intros kn n params PAll.
-        case (find (fun '(kn',_) => eq_kername kn kn') global_adt).
-        + intros [_ Hrel]. 
-          refine (to_realize_term (Hrel params _ n)).
-          induction PAll; econstructor; eauto. eapply to_realize_value; eassumption.
-        + intros; exact False. 
-    Defined.
-
-    Definition realize_value (A:camlType) : value -> Prop :=
-      to_realize_value (realize_term A).
-
-  End Values. 
-  MetaCoq Quote Recursively Definition tnat := nat.
-
-  Fixpoint realize_ADT_gen_fix (global_adt : global_adt_decl) 
-    (adt : list (list (list camlType))) (step : nat) : realize_adt_type.
-  Proof.
-    destruct step; [compute; intros; exact False|].
-    intros params paramRel ind. 
-    destruct (Nat.ltb ind (List.length adt)); [|intros; exact False].
-    pose proof (constr_list := List.nth ind adt []). 
-    refine (fun v => _\/_).
-    - pose (constr_noarg := filter 
-      (fun x => match x with [] => true 
-            | _ => false end) constr_list).
-      refine (Existsi (fun index Ts => v = value_Int (Int , Z.of_nat index)) 0 constr_noarg).
-    - pose (constr_arg := filter 
-      (fun x => match x with [] => false 
-          | _ => true end) constr_list).
-      refine (Existsi (fun index Ts => 
-          exists vs, v = Block (int_of_nat index, vs) /\ _) 0 constr_arg). 
-      refine (Forall2 (realize_value _ global_adt) Ts vs).
-      refine (_ ++ _).
-      + (* parameters *)
-        clear -paramRel. induction paramRel; [exact []| ].
-        refine (p :: IHparamRel).
-      + (* recursive calls *)
-        exact (to_list (realize_ADT_gen_fix global_adt adt step params paramRel) (List.length adt)).
-  Defined.   
-
-  Definition realize_ADT_gen (global_adt : global_adt_decl) 
-    : ADT -> nat -> realize_adt_type :=
-    fun '(n , adt) step params =>
-      if (Nat.eqb n (List.length params)) 
-      then realize_ADT_gen_fix global_adt adt step params
-      else fun _ _ _ => False.
-
-  Definition realize_ADT (global_adt : global_adt_decl) : ADT -> realize_adt_type :=
-    fun adt params paramRel ind v => exists n, realize_ADT_gen global_adt adt n params paramRel ind v.
-
-  Definition add_ADT (global_adt : global_adt_decl) (kn : kername) (adt : ADT) :  global_adt_decl := 
-    (kn, realize_ADT global_adt adt) :: global_adt.
-
-End Realizability.
 
 Section firstorder.
 
@@ -463,78 +316,6 @@ ind_universes0 ind_variance0) x Hparam Hfo'); eauto.
     ind_params mind = [] -> 
     is_true (forallb (@firstorder_oneind Σb mind) (ind_bodies mind)) -> ADT :=
     fun Hparam H => (0, CoqType_to_camlType' mind Hparam H).
-
-  Definition empty_heap : CanonicalHeap.(heapGen) (@SemanticsSpec.value CanonicalHeap) :=
-    (int_of_nat 0 , fun _ => []).
-
-  Lemma lookup_inductive_env Σ kn Emind Eind ind :
-    EGlobalEnv.lookup_inductive Σ (mkInd kn ind) = Some (Emind,Eind) ->
-    EGlobalEnv.lookup_env Σ kn = Some (EAst.InductiveDecl Emind).
-  Proof.
-    induction Σ; cbn; intros.
-    - inversion H.
-    - destruct (ReflectEq.eqb kn (fst a)); cbn in *.
-      + f_equal. destruct (snd a); cbn in *; [inversion H|].
-        destruct (nth_error (EAst.ind_bodies m) ind); now inversion H.  
-      + apply IHΣ; eauto.
-  Qed.
-                  
-  Fixpoint zip {A B} (l:list A) (l':list B) : list (A * B) :=
-  match l , l' with 
-  | [] , [] => []
-  | a::l , b::l' => ((a,b) :: zip l l')
-  | _ , _ => [] 
-  end. 
-    
-  Lemma zip_length {A B} (l:list A) (l':list B) : 
-    #|l| = #|l'| ->  #|zip l l'| = #|l|.
-  Proof. 
-    revert l'; induction l; destruct l'; cbn; eauto.
-    intro Heq; inversion Heq. rewrite IHl; eauto.  
-  Qed. 
-
-  Lemma zip_fst {A B} (l:list A) (l':list B) : 
-    #|l| = #|l'| -> map fst (zip l l') = l.
-  revert l'; induction l; destruct l'; cbn; eauto.
-  - inversion 1.
-  - intro Heq; inversion Heq. rewrite IHl; eauto.
-  Qed.         
-
-  Lemma zip_snd {A B} (l:list A) (l':list B) : 
-  #|l| = #|l'| -> map snd (zip l l') = l'.
-  revert l'; induction l; destruct l'; cbn; eauto.
-  - inversion 1.  
-  - intro Heq; inversion Heq. rewrite IHl; eauto.
-  Qed.  
-
-  Fixpoint All_exists T U A P l l'
-    (H: Forall2 (fun (t : T) (u : U) => exists a : A, P t u a) l l')  
-    : exists l'' : list A, Forall2 (fun tu a => P (fst tu) (snd tu) a) (zip l l') l''.
-  Proof. 
-    destruct H.
-    - exists []. econstructor.
-    - destruct H as [p H].
-      refine (let '(ex_intro l' X) := 
-              All_exists T U A P _ _ H0 in _).
-      exists (p::l'). econstructor; eauto. 
-  Qed. 
-
-  Lemma Forall2_acc_cst (X A B : Type) (R : X -> A -> X -> B -> Prop) x l l' :
-    Forall2 (fun a b => R x a x b) l l' -> Forall2_acc R x l x l'.
-  Proof.
-    induction 1; econstructor; eauto.
-  Qed.
-
-  Lemma Forall2_sym :
-  forall A B (P : A -> B -> Prop) l l',
-    Forall2 P l l' ->
-    Forall2 (fun x y => P y x) l' l.
-  Proof.
-  intros A B P l l' h.
-  induction h.
-  - constructor.
-  - constructor. all: auto.
-  Qed.
   
   Lemma CoqType_to_camlType_ind_ctors_nth 
     mind ind_ctors Hparam a k i :
@@ -591,22 +372,6 @@ ind_universes0 ind_variance0) x Hparam Hfo'); eauto.
       + cbn in *. now eapply IHind_ctors0. 
   Qed. 
 
-  Lemma Forall_Forall2_and_inv {A B : Type} 
-    {R : A -> B -> Prop} {P : A -> Prop} l l':
-  Forall2 (fun (x : A) (y : B) => P x /\ R x y ) l l' ->
-  Forall2 R l l' /\ Forall P l.
-  Proof. 
-    induction 1; repeat econstructor; now eauto.
-  Qed.
-
-  Lemma Forall2_forall {A B X: Type} 
-    {R : A -> B -> X -> Prop} l l':
-  Forall2 (fun a b => forall x, R a b x) l l' ->
-  forall x, Forall2 (fun a b => R a b x) l l'.
-  Proof.
-    induction 1; econstructor; eauto.
-  Qed.
-
   Axiom ctors_max_length : forall mind j k ind ctors,
     nth_error mind j = Some ind ->
     nth_error (ind_ctors ind) k = Some ctors -> 
@@ -616,14 +381,6 @@ ind_universes0 ind_variance0) x Hparam Hfo'); eauto.
     #|ind_ctors ind| <= Z.to_nat Uint63.wB.
 
   Axiom compile_pipeline : global_declarations -> term -> t.
-
-  Definition cstr_nargs : constructor_body -> nat := fun c => #| cstr_args c|.
-
-  Definition lookup_constructor_args Σ ind : option (list nat) 
-    := match lookup_inductive Σ ind with
-    | Some (_, idecl) => Some (map cstr_nargs (ind_ctors idecl))
-   | None => None
-    end.
 
   Axiom compile_pipeline_tConstruct_nil : forall Σ i n inst, 
     compile_pipeline Σ.(declarations) (tConstruct i n inst) = 
@@ -724,15 +481,6 @@ ind_universes0 ind_variance0) x Hparam Hfo'); eauto.
         * intros; f_equal. eapply IHind_ctors0; eauto.
     - now eapply nth_error_Some_length. 
   Qed. 
-
-  Lemma Forall2_map_left {A B C} (P : A -> B -> Prop) (f : C -> A) (l : list C) (l' : list B) :
-    Forall2 P (map f l) l' <-> Forall2 (fun x y => P (f x) y) l l'.
-Proof.
-  split; intros.
-  + eapply Forall2_map_inv. now rewrite map_id.
-  + rewrite -(map_id l'). now eapply Forall2_map.
-Qed.
-
 End firstorder.
 
 Lemma CoqType_to_camlType_oneind_type_Rel n k decl_type Hfo :
@@ -850,33 +598,6 @@ Proof.
   edestruct e as [i [? [? ?]]]; eauto. exists (i - k). repeat split; eauto.
   all: lia.
 Qed.
-
-Inductive Forall2i {A B : Type} (R : nat -> A -> B -> Prop) (n : nat)
-  : list A -> list B -> Prop :=
-| Forall2i_nil : Forall2i R n [] []
-| Forall2i_cons :
-    forall x y l r,
-      R n x y ->
-      Forall2i R (S n) l r ->
-      Forall2i R n (x :: l) (y :: r).
-Arguments Forall2i_nil {_ _ _ _}.
-Arguments Forall2i_cons {_ _ _ _ _ _ _ _}.
-
-Derive Signature NoConfusionHom for All2i.
-
-Lemma Forall2_Forall_mix {A B} {P : B -> Prop} {Q : A -> B -> Prop}
-   {l : list A} {l' : list B} :
-  Forall2 (fun x y => (P y -> Q x y)) l l' -> Forall P l' -> Forall2 Q l l'.
-Proof.
-  induction 1; simpl; intros; constructor; inversion H1; eauto.
-Qed.
-
-  Lemma Forall2_and_inv {A B : Type} (R R' : A -> B -> Prop) (l : list A) (l' : list B) :
-    Forall2 (fun (x : A) (y : B) => R x y /\ R' x y) l l'
-    -> Forall2 R l l' /\ Forall2 R' l l'.
-  Proof.
-    induction 1; split; eauto; econstructor; destruct H; now destruct IHForall2.
-  Qed.
 
   Inductive nonDepProd : term -> Type :=
     | nonDepProd_tInd : forall i u, nonDepProd (tInd i u)
@@ -1025,7 +746,7 @@ Proof.
     realize_ADT _ [] [] adt [] All_nil ind v ->
     exists t, forall h,  
     ∥ (Σ , univ_decl) ;;; [] |- t : tInd (mkInd kn ind) [] ∥ /\ 
-    eval _ [] (empty_locals _) h (compile_pipeline Σ.(declarations) t) h v.
+    eval [] (empty_locals _) h (compile_pipeline Σ.(declarations) t) h v.
   Proof. 
     rename H into HHeap; rename H0 into H. 
     intros adt Σ wfΣ Hflag v ind Eind Hind Hlookup [step Hrel].
@@ -1146,7 +867,7 @@ Proof.
         subst.
         assert (Forall2 (fun v T => 
         (exists t, forall h,  ∥ (Σ , univ_decl) ;;; [] |- fst t : tInd (mkInd kn (#|ind_bodies mind| - S (snd t))) [] ∥ /\ 
-        eval _ [] (empty_locals _) h (compile_pipeline Σ.(declarations) (fst t)) h v
+        eval [] (empty_locals _) h (compile_pipeline Σ.(declarations) (fst t)) h v
         /\ (0 <= snd t) /\ (snd t < #|ind_bodies mind|) /\ T = Rel (#|ind_bodies mind| - S (snd t)))) v' (T::Ts)).
         { 
           assert (Forall (fun T => exists l l', In (l ++ [T] ++ l') (nth ind (CoqType_to_camlType' mind Hparam Hfo) [])) (T::Ts)).
@@ -1215,7 +936,7 @@ Proof.
             rewrite <- (map_id v'). apply Forall2_map. 
             rewrite Forall2_map_left. 
             erewrite <- (Forall2_map_right (fun a b =>
-            eval HHeap [] (empty_locals HHeap) h
+            eval [] (empty_locals HHeap) h
               (compile_pipeline [(kn, InductiveDecl mind)]
                  (fst a)) h b) fst) in Heval.
             rewrite zip_fst in Heval; eauto. 
@@ -1318,169 +1039,22 @@ Proof.
     lookup_inductive Σ (mkInd kn ind) = Some (mind, Eind) ->
     ∥ (Σ , univ_decl) ;;; [] |- t : tInd (mkInd kn ind) [] ∥ ->
     forall h v, 
-      eval _ [] (empty_locals _) h (compile_pipeline Σ.(declarations) t) h v
+      eval [] (empty_locals _) h (compile_pipeline Σ.(declarations) t) h v
       -> realize_ADT _ [] [] adt [] All_nil ind v.
   Proof.
   Admitted.  
 
-  From Malfunction Require Import CompileCorrect Pipeline.
-
-  Section fix_global.
-
-  Variable Σ : list Ident.t.
-
-  Fixpoint isPure (t : t) :=
-    match t with
-    | Mvar x => true
-    | Mlambda (ids, x) => isPure x
-    | Mapply (x, args) => isPure x && forallb isPure args
-    | Mlet (binds, x) => forallb isPure_binding binds && isPure x
-    | Mnum x => true
-    | Mstring x => false (* strings are interpreted using vectors *)
-    | Mglobal id => true
-    | Mswitch (x, sels) => isPure x && forallb (fun '(_, x) => isPure x) sels
-    | Mnumop1 (op, num, x) => isPure x
-    | Mnumop2 (op, num, x1, x2) => isPure x1 && isPure x2
-    | Mconvert (from, to, x) => isPure x
-    | Mblock (tag, xs) => forallb isPure xs
-    | Mfield (i, x) => isPure x
-    | _ => false
-    end
-  with isPure_binding (b : binding) :=
-         match b with
-         | Unnamed x => isPure x
-         | Named (id, x) => isPure x
-         | Recursive recs => forallb (fun '(id,x) => isPure x) recs
-         end.
-
-  Definition isPure_rec_value `{Heap} (v : rec_value) :=
-    match v with 
-    | RFunc (_ , t) => is_true (isPure t)
-    | Bad_recursive_value => True
-    | _ => False
-    end. 
-
-  Fixpoint isPure_value `{Heap} (v : value) {struct v} :=
-    match v with
-    | Block (_,vs) => Forall (fun p => p) (map isPure_value vs)
-    | Func (locals,_,t) => (forall s, isPure_value (locals s)) /\ is_true (isPure t)    
-    | RClos (locals,self,mfix,t) => (forall s, isPure_value (locals s)) /\ Forall isPure_rec_value mfix
-    | value_Int _ => True
-    | Float _ => True
-    | fail _ => True
-    | _ => False
-    end.
-
-End fix_global.
-
-Lemma isPure_add_self `{Heap} locals mfix self s :
-  (forall s : Ident.t, isPure_value (locals s)) ->
-  Forall isPure_rec_value mfix ->
-  isPure_value (add_self self mfix locals s).
-Proof.
-  intros Hlocals Hmfix. unfold add_self, add_recs, List.mapi.
-  generalize 0 as i. generalize self at 1. 
-  induction self; cbn; eauto.
-  unfold Ident.Map.add. destruct (Ident.eqb s a); cbn; eauto.
-Qed.
-
-Lemma isPure_heap `{Heap} `{WcbvFlags} locals h h' t v :
-  is_true (isPure t) ->
-  (forall s, isPure_value (locals s)) -> 
-  eval [] locals h t h' v -> isPure_value v /\ h = h'.
-Proof.
-  intros Hpure Hlocals. induction 1; try solve [inversion Hpure]; cbn in Hpure;
-  repeat rewrite MCProd.andb_and in Hpure; try solve [cbn; repeat split; eauto]; eauto. 
-  - cbn in *. destruct Hpure as [? [? ?]].
-    try (destruct IHeval1; eauto);
-     try (destruct IHeval2; eauto); try (destruct IHeval3; eauto); try now eauto.
-    destruct H4. intros s. unfold Ident.Map.add. destruct (Ident.eqb s x); eauto.
-  - destruct Hpure as [? [? ?]].
-    try (destruct IHeval1; eauto);
-     try (destruct IHeval2; eauto); try (destruct IHeval3; eauto); try now eauto.
-    destruct H5. pose proof (proj1 (Forall_nth _ _) H9 n Bad_recursive_value). rewrite H1 in H10.
-    eapply H10. case_eq (Nat.ltb n #|mfix|); try rewrite Nat.ltb_lt; eauto.
-    rewrite Nat.ltb_ge. intro neq.  rewrite nth_overflow in H1; eauto. inversion H1.  
-    destruct H5. intros s. unfold Ident.Map.add. destruct (Ident.eqb s y); eauto.
-    eapply isPure_add_self; eauto. 
-  - cbn in *. destruct Hpure as [? [? ?]]; try (destruct IHeval1; eauto); now eauto.
-  - destruct Hpure as [? [? [? ?]]]. repeat rewrite MCProd.andb_and in IHeval.
-    destruct IHeval ; eauto.
-  - cbn in *. destruct Hpure as [[? ?] ?]; try (destruct IHeval1; eauto); try (destruct IHeval2; eauto); now eauto.  
-  - cbn in *. destruct Hpure as [[? ?] ?]; try (destruct IHeval1; eauto); try (destruct IHeval2; eauto); try now eauto.
-    intros s. unfold Ident.Map.add. destruct (Ident.eqb s x); eauto.
-  - cbn in *. destruct Hpure as [[? ?] ?]; try (destruct IHeval; eauto); try now eauto.
-    intros s. rewrite H1. eapply isPure_add_self; eauto. unfold rfunc, RFunc_build.
-    eapply forallb_Forall in H3. clear -H3. induction recs; eauto; cbn. destruct a; cbn in *. inversion H3; subst.
-    econstructor; eauto. destruct t0; cbn; eauto. destruct p. cbn in H2. destruct l; cbn ; eauto.
-    destruct l; cbn ; eauto.
-  - cbn in *. destruct Hpure as [? ?]; try (destruct IHeval1; eauto); try (destruct IHeval2; eauto); try now eauto.
-    induction cases; cbn in *. inversion H1. repeat rewrite MCProd.andb_and in H3. destruct H3.   
-    destruct a. destruct (existsb _ _); [inversion H1; subst; eauto|]. now eapply IHcases.
-  - cbn in *. clear H1 H2. induction H3; [now eauto|]. repeat rewrite MCProd.andb_and in Hpure.
-    destruct Hpure. destruct IHForall2_acc; eauto. destruct H1; eauto. cbn; split; now eauto.
-  - cbn in *. destruct IHeval; eauto. split; eauto. eapply Forall_nth; eauto. now eapply Forall_map_inv in H4.
-  - cbn in *. now eauto.
-  - cbn in *. inversion H1.
-  - cbn in *. destruct IHeval; eauto.
-  - cbn. destruct Hpure. destruct IHeval1; eauto. destruct IHeval2; eauto. now destruct op.
-  - cbn; now eauto.   
-  - cbn; destruct Hpure. destruct IHeval1; eauto. destruct IHeval2; now eauto.
-  - cbn; destruct Hpure. destruct IHeval1; eauto. destruct IHeval2; now eauto.
-  - cbn; destruct IHeval; eauto. 
-  - cbn. destruct IHeval; eauto.
-  - cbn. destruct IHeval; eauto.
-Qed.            
-
-Lemma isPure_heap_irr `{Heap} `{WcbvFlags} h h' locals t v :
-  is_true (isPure t) ->
-  (forall s, isPure_value (locals s)) -> 
-  eval [] locals h t h' v -> forall h'', eval [] locals h'' t h'' v.
-Proof.
-  intros Hpure Hlocals. induction 1; try solve [inversion Hpure]; cbn in Hpure;
-  repeat rewrite MCProd.andb_and in Hpure; try solve [cbn; destruct Hpure; econstructor; eauto]; 
-  try solve [cbn; econstructor; eauto].
-  - intro. destruct Hpure as [? [? ?]]. econstructor 3; eauto.
-    eapply isPure_heap in H1_, H1_0; eauto. destruct H1_ as [[Hlocals' He] _].  
-    eapply IHeval3; eauto. intros s. unfold Ident.Map.add. destruct (Ident.eqb s x); now eauto.
-  - intro. destruct Hpure as [? [? ?]]. econstructor 4; eauto.
-    eapply isPure_heap in H1_, H1_0; eauto. destruct H1_ as [[Hlocals' He] _].
-    pose proof (proj1 (Forall_nth _ _) He n Bad_recursive_value).
-    rewrite H1 in H5. cbn in H5. eapply IHeval3.
-    case_eq (Nat.ltb n #|mfix|); try rewrite Nat.ltb_lt; eauto.
-    rewrite Nat.ltb_ge. intro neq. rewrite nth_overflow in H1; eauto. inversion H1.  
-    destruct H1_0. intros s. unfold Ident.Map.add. destruct (Ident.eqb s y); eauto.
-    eapply isPure_add_self; eauto. 
-  - intro. destruct Hpure as [? [? ?]]. econstructor 6; eauto.
-    eapply IHeval; eauto. cbn. now repeat rewrite MCProd.andb_and.
-  - intro. destruct Hpure as [[? ?] ?]. econstructor; eauto. eapply IHeval2; eauto. 
-    cbn. now repeat rewrite MCProd.andb_and.
-  - intro. destruct Hpure as [[? ?] ?]. econstructor; eauto. eapply IHeval2; eauto. 
-    cbn. now repeat rewrite MCProd.andb_and. 
-    intros s. unfold Ident.Map.add. destruct (Ident.eqb s x); eauto. eapply isPure_heap in H1_; now eauto. 
-  - intro. destruct Hpure as [[? ?] ?]. econstructor; eauto. rewrite H1 in IHeval. eapply IHeval; eauto; cbn.
-    now repeat rewrite MCProd.andb_and. intro s. eapply isPure_add_self; eauto.
-    unfold rfunc, RFunc_build.
-    eapply forallb_Forall in H3. clear -H3. induction recs; eauto; cbn. destruct a; cbn in *. inversion H3; subst.
-    econstructor; eauto. destruct t0; cbn; eauto. destruct p. cbn in H2. destruct l; cbn ; eauto.
-    destruct l; cbn ; eauto. 
-  - destruct Hpure. econstructor; eauto. eapply IHeval2; eauto.   
-    induction cases; cbn in *. inversion H1. repeat rewrite MCProd.andb_and in H3. destruct H3.   
-    destruct a. destruct (existsb _ _); [inversion H1; subst; eauto|]. now eapply IHcases.
-  - econstructor; eauto. clear H1 H2. induction H3; [econstructor; eauto|].
-    cbn in Hpure. rewrite MCProd.andb_and in Hpure. destruct Hpure. econstructor; eauto.
-Qed. 
+From Malfunction Require Import CompileCorrect Pipeline. 
 
 Axiom compile_pure : forall `{Heap} `{WcbvFlags} Σ t, is_true (isPure (compile_pipeline Σ t)).
 
-Axiom compile_compose : forall `{Heap} `{WcbvFlags} (cf:=config.extraction_checker_flags) 
-  (Σ:global_env) univ_decl h h' t u' u v w na A B,
+Axiom compile_app : forall `{Heap} `{WcbvFlags} 
+  (cf:=config.extraction_checker_flags) 
+  (Σ:global_env) univ_decl t u na A B,
   ∥ (Σ , univ_decl) ;;; [] |- t : tProd na A B ∥ ->
   ~ ∥Extract.isErasable (Σ , univ_decl) [] t∥ -> 
-  eval [] (empty_locals _) h (compile_pipeline Σ.(declarations) u) h v ->
-  eval [] (empty_locals _) h u' h' v ->
-  eval [] (empty_locals _) h (Mapply (compile_pipeline Σ.(declarations) t, [u'])) h' w ->
-  eval [] (empty_locals _) h (compile_pipeline Σ.(declarations) (tApp t u)) h w.
+  compile_pipeline Σ.(declarations) (tApp t u) = 
+  Mapply (compile_pipeline Σ.(declarations) t, [compile_pipeline Σ.(declarations) u]).
 
 Axiom compile_function : forall `{Heap} `{WcbvFlags} (cf:=config.extraction_checker_flags)
   Σ univ_decl h h' f v na A B,
@@ -1488,6 +1062,41 @@ Axiom compile_function : forall `{Heap} `{WcbvFlags} (cf:=config.extraction_chec
   ~ ∥Extract.isErasable (Σ , univ_decl) [] f∥ ->
   eval [] (empty_locals _) h (compile_pipeline Σ.(declarations) f) h' v ->
   isFunction v = true.
+
+Lemma compile_compose `{Heap} `{WcbvFlags} (cf:=config.extraction_checker_flags) 
+  (Σ:global_env) univ_decl h h' t u' u v w na A B :
+  ∥ (Σ , univ_decl) ;;; [] |- t : tProd na A B ∥ ->
+  ~ ∥Extract.isErasable (Σ , univ_decl) [] t∥ -> 
+  eval [] (empty_locals _) h (compile_pipeline Σ.(declarations) u) h v ->
+  eval [] (empty_locals _) h u' h' v ->
+  eval [] (empty_locals _) h (Mapply (compile_pipeline Σ.(declarations) t, [u'])) h' w ->
+  eval [] (empty_locals _) h (compile_pipeline Σ.(declarations) (tApp t u)) h w.
+Proof.
+  intros Htyp Herase Hu Hu' Happ.
+  erewrite compile_app; eauto.
+  inversion Happ; subst. 
+  - epose proof (compile_pure _ t).
+    eapply isPure_heap in H1 as [Hfpure heq]; eauto.
+    2: intros; cbn; eauto. symmetry in heq; subst. 
+    econstructor 3; eauto.
+    assert (v = v2) by apply todo. symmetry in H1; subst.
+    eapply isPure_heap in Hu as [Hvpure _]; try eapply compile_pure; intros; cbn; eauto.
+    destruct Hfpure as [? Hepure]. eapply isPure_heap_irr; eauto.
+    intro. unfold Ident.Map.add. destruct (Ident.eqb s x); eauto.
+  - epose proof (compile_pure _ t).
+    eapply isPure_heap in H1 as [Hfpure heq]; eauto.
+    2: intros; cbn; eauto. symmetry in heq; subst.  
+    econstructor 4; eauto.
+    assert (v = v2) by apply todo. symmetry in H1; subst.
+    eapply isPure_heap in Hu as [Hvpure _]; try eapply compile_pure; intros; cbn; eauto.
+    destruct Hfpure as [? Hepure]. eapply isPure_heap_irr; eauto.
+    2: { intro. unfold Ident.Map.add. destruct (Ident.eqb s y); eauto. 
+         eapply isPure_add_self; eauto. }
+    rewrite nth_nth_error in H6.
+    eapply (nth_error_forall (n:=n) (x:=RFunc (y, e))) in Hepure; eauto.  
+    destruct nth_error; [now f_equal |inversion H6].
+  - erewrite compile_function in H7; eauto. inversion H7.
+Qed.  
 
 Lemma CoqFunction_to_CamlFunction `{Heap} `{WcbvFlags} (cf:=config.extraction_checker_flags)
     univ retro univ_decl kn mind 
@@ -1558,7 +1167,8 @@ Proof.
     unshelve eapply camlValue_to_CoqValue_nil in Ht; eauto; cbn.
     destruct Ht as [t_coq Ht]. specialize (Ht h2). destruct Ht as [Ht_typ Ht_eval].
     assert (h2 = h').
-    { eapply isPure_heap in H6; try eapply compile_pure; intros; cbn; eauto. cbn in H6. destruct H6 as [[? ? ] ?]. 
+    { eapply isPure_heap in H6; try eapply compile_pure; intros; cbn; eauto. cbn in H6.
+      destruct H6 as [[? ? ] ?]. 
       eapply isPure_heap; try apply H11; intros; cbn; eauto.
       unfold Ident.Map.add. destruct (Ident.eqb s x); eauto.
       eapply isPure_heap in Ht_eval; try eapply compile_pure; intros; cbn; eauto. now destruct Ht_typ. }
