theories/RealizabilitySemantics.v
@@ -1,0 +1,439 @@
+Require Import ssreflect ssrbool Eqdep_dec.
+From Equations Require Import Equations. 
+From MetaCoq.Utils Require Import All_Forall MCSquash MCList.
+From MetaCoq.Common Require Import Transform config Kernames.
+From MetaCoq.PCUIC Require Import PCUICAst PCUICTyping PCUICFirstorder PCUICCasesHelper BDStrengthening PCUICCumulativity.
+From MetaCoq.Erasure Require Import EWcbvEval EWcbvEvalNamed.
+From MetaCoq.SafeChecker Require Import PCUICErrors PCUICWfEnv PCUICWfEnvImpl.
+
+From Malfunction Require Import Malfunction SemanticsSpec utils_array Compile.
+
+Require Import ZArith Array.PArray List String Floats Lia Bool.
+Import ListNotations.
+From MetaCoq.Utils Require Import bytestring.
+
+Unset Elimination Schemes. 
+
+Inductive camlType : Set :=
+    Arrow : camlType -> camlType -> camlType
+  | Rel : nat -> camlType
+  | Adt : kername -> 
+            (* number of the ADT in the mutual definition *) nat -> 
+            (* list of parameters *) list camlType -> 
+            camlType.
+
+Definition camlType_rect :
+forall P : camlType -> Type,
+       (forall c : camlType,
+        P c -> forall c0 : camlType, P c0 -> P (Arrow c c0)) ->
+       (forall n : nat, P (Rel n)) ->
+       (forall (k : kername) i (l : list camlType), All P l -> P (Adt k i l)) ->
+       forall c : camlType, P c. 
+Proof. 
+  intros P X X0 X1. fix f 1. intros c; destruct c.
+  - eapply X; eauto.   
+  - eapply X0; eauto. 
+  - eapply X1; eauto. induction l; econstructor; eauto. 
+Defined.
+       
+Set Elimination Schemes. 
+
+Notation "A → B" := (Arrow A B) (at level 50). 
+
+Definition isArrow T := match T with Arrow _ _ => true | _ => false end.
+
+Definition ADT : Set := 
+  (* number of parameters *)
+  nat * list (
+    list (list camlType) (* list of constructors for each ADT *)).
+
+Inductive Existsi {A : Type} (P : nat -> A -> Prop) (n : nat) 
+  : list A -> Prop :=
+	  Existsi_cons_hd : forall x l, P n x -> Existsi P n (x :: l)
+  | Existsi_cons_tl : forall (x : A) (l : list A),
+                     Existsi P (S n) l -> Existsi P n (x :: l).
+
+Lemma Existsi_spec A (P : nat -> A -> Prop) n (l:list A) : Existsi P n l -> 
+  exists k x, n <= k /\ k < n + List.length l /\ P k x /\ nth_error l (k-n) = Some x.
+Proof.
+  induction 1.
+  - exists n; exists x. cbn; repeat split; eauto. lia.
+    now rewrite Nat.sub_diag.   
+  - destruct IHExistsi as [k [a [Hk [Hk' [HP Ha]]]]].
+    exists k; exists a. repeat split; eauto; cbn; try lia.
+    assert (k - n = S (k - S n)) by lia.
+    now rewrite H0. 
+Defined. 
+
+Section Realizability. 
+
+  Variable _Heap:Heap.
+
+  Definition realize_adt_type := 
+      forall (params: list camlType), All (fun _ => value -> Prop) params -> 
+              ((* number of the ADT in the mutual definition *) nat -> value -> Prop).
+
+  Variable globals : list (Ident.t * value).
+  
+  Definition global_adt_decl := list (kername * realize_adt_type).
+
+  Open Scope bs. 
+
+  Definition empty_locals : Ident.Map.t := fun _ => fail "not_defined".
+
+  Close Scope bs. 
+
+  Section Values. 
+
+    Variable local_adt : list (value -> Prop).
+    Variable global_adt : global_adt_decl.
+
+    Definition to_realize_term (realize_val : value -> Prop) 
+      : t -> Prop := fun t => forall h h' v, 
+      eval _ globals empty_locals h t h' v -> realize_val v.
+
+    Definition to_realize_value (realize_term : t -> Prop) 
+      : value -> Prop := fun v => exists t h h', 
+        eval _ globals empty_locals h t h' v /\ realize_term t.
+
+    Definition realize_term (A:camlType) : t -> Prop.
+    Proof.
+      refine (camlType_rect _ _ _ _ A); clear A.
+      - intros A PA B PB.
+        exact (fun f => forall t, PA t -> PB (Mapply(f,[t]))).
+      - intros n. 
+        exact (to_realize_term (List.nth n local_adt (fun _ => False))).
+      - intros kn n params PAll.
+        case (find (fun '(kn',_) => eq_kername kn kn') global_adt).
+        + intros [_ Hrel]. 
+          refine (to_realize_term (Hrel params _ n)).
+          induction PAll; econstructor; eauto. eapply to_realize_value; eassumption.
+        + intros; exact False. 
+    Defined.
+
+    Definition realize_value (A:camlType) : value -> Prop :=
+      to_realize_value (realize_term A).
+
+  End Values. 
+  MetaCoq Quote Recursively Definition tnat := nat.
+
+  Fixpoint realize_ADT_gen_fix (global_adt : global_adt_decl) 
+    (adt : list (list (list camlType))) (step : nat) : realize_adt_type.
+  Proof.
+    destruct step; [compute; intros; exact False|].
+    intros params paramRel ind. 
+    destruct (Nat.ltb ind (List.length adt)); [|intros; exact False].
+    pose proof (constr_list := List.nth ind adt []). 
+    refine (fun v => _\/_).
+    - pose (constr_noarg := filter 
+      (fun x => match x with [] => true 
+            | _ => false end) constr_list).
+      refine (Existsi (fun index Ts => v = value_Int (Int , Z.of_nat index)) 0 constr_noarg).
+    - pose (constr_arg := filter 
+      (fun x => match x with [] => false 
+          | _ => true end) constr_list).
+      refine (Existsi (fun index Ts => 
+          exists vs, v = Block (int_of_nat index, vs) /\ _) 0 constr_arg). 
+      refine (Forall2 (realize_value _ global_adt) Ts vs).
+      refine (_ ++ _).
+      + (* parameters *)
+        clear -paramRel. induction paramRel; [exact []| ].
+        refine (p :: IHparamRel).
+      + (* recursive calls *)
+        exact (to_list (realize_ADT_gen_fix global_adt adt step params paramRel) (List.length adt)).
+  Defined.   
+
+  Definition realize_ADT_gen (global_adt : global_adt_decl) 
+    : ADT -> nat -> realize_adt_type :=
+    fun '(n , adt) step params =>
+      if (Nat.eqb n (List.length params)) 
+      then realize_ADT_gen_fix global_adt adt step params
+      else fun _ _ _ => False.
+
+  Definition realize_ADT (global_adt : global_adt_decl) : ADT -> realize_adt_type :=
+    fun adt params paramRel ind v => exists n, realize_ADT_gen global_adt adt n params paramRel ind v.
+
+  Definition add_ADT (global_adt : global_adt_decl) (kn : kername) (adt : ADT) :  global_adt_decl := 
+    (kn, realize_ADT global_adt adt) :: global_adt.
+
+End Realizability.
+
+
+  Definition empty_heap : CanonicalHeap.(heapGen) (@SemanticsSpec.value CanonicalHeap) :=
+    (int_of_nat 0 , fun _ => []).
+
+  Lemma lookup_inductive_env Σ kn Emind Eind ind :
+    EGlobalEnv.lookup_inductive Σ (mkInd kn ind) = Some (Emind,Eind) ->
+    EGlobalEnv.lookup_env Σ kn = Some (EAst.InductiveDecl Emind).
+  Proof.
+    induction Σ; cbn; intros.
+    - inversion H.
+    - destruct (ReflectEq.eqb kn (fst a)); cbn in *.
+      + f_equal. destruct (snd a); cbn in *; [inversion H|].
+        destruct (nth_error (EAst.ind_bodies m) ind); now inversion H.  
+      + apply IHΣ; eauto.
+  Qed.
+                  
+  Fixpoint zip {A B} (l:list A) (l':list B) : list (A * B) :=
+  match l , l' with 
+  | [] , [] => []
+  | a::l , b::l' => ((a,b) :: zip l l')
+  | _ , _ => [] 
+  end. 
+    
+  Lemma zip_length {A B} (l:list A) (l':list B) : 
+    #|l| = #|l'| ->  #|zip l l'| = #|l|.
+  Proof. 
+    revert l'; induction l; destruct l'; cbn; eauto.
+    intro Heq; inversion Heq. rewrite IHl; eauto.  
+  Qed. 
+
+  Lemma zip_fst {A B} (l:list A) (l':list B) : 
+    #|l| = #|l'| -> map fst (zip l l') = l.
+  revert l'; induction l; destruct l'; cbn; eauto.
+  - inversion 1.
+  - intro Heq; inversion Heq. rewrite IHl; eauto.
+  Qed.         
+
+  Lemma zip_snd {A B} (l:list A) (l':list B) : 
+  #|l| = #|l'| -> map snd (zip l l') = l'.
+  revert l'; induction l; destruct l'; cbn; eauto.
+  - inversion 1.  
+  - intro Heq; inversion Heq. rewrite IHl; eauto.
+  Qed.  
+
+  Fixpoint All_exists T U A P l l'
+    (H: Forall2 (fun (t : T) (u : U) => exists a : A, P t u a) l l')  
+    : exists l'' : list A, Forall2 (fun tu a => P (fst tu) (snd tu) a) (zip l l') l''.
+  Proof. 
+    destruct H.
+    - exists []. econstructor.
+    - destruct H as [p H].
+      refine (let '(ex_intro l' X) := 
+              All_exists T U A P _ _ H0 in _).
+      exists (p::l'). econstructor; eauto. 
+  Qed. 
+
+  Lemma Forall2_acc_cst (X A B : Type) (R : X -> A -> X -> B -> Prop) x l l' :
+    Forall2 (fun a b => R x a x b) l l' -> Forall2_acc R x l x l'.
+  Proof.
+    induction 1; econstructor; eauto.
+  Qed.
+
+  Lemma Forall2_sym :
+  forall A B (P : A -> B -> Prop) l l',
+    Forall2 P l l' ->
+    Forall2 (fun x y => P y x) l' l.
+  Proof.
+  intros A B P l l' h.
+  induction h.
+  - constructor.
+  - constructor. all: auto.
+  Qed.
+  
+ Lemma Forall_Forall2_and_inv {A B : Type} 
+  {R : A -> B -> Prop} {P : A -> Prop} l l':
+    Forall2 (fun (x : A) (y : B) => P x /\ R x y ) l l' ->
+    Forall2 R l l' /\ Forall P l.
+  Proof. 
+    induction 1; repeat econstructor; now eauto.
+  Qed.
+
+  Lemma Forall2_forall {A B X: Type} 
+    {R : A -> B -> X -> Prop} l l':
+  Forall2 (fun a b => forall x, R a b x) l l' ->
+  forall x, Forall2 (fun a b => R a b x) l l'.
+  Proof.
+    induction 1; econstructor; eauto.
+  Qed.
+
+  Definition cstr_nargs : constructor_body -> nat := fun c => #| cstr_args c|.
+
+  Lemma Forall2_map_left {A B C} (P : A -> B -> Prop) (f : C -> A) (l : list C) (l' : list B) :
+    Forall2 P (map f l) l' <-> Forall2 (fun x y => P (f x) y) l l'.
+  Proof.
+    split; intros.
+    + eapply Forall2_map_inv. now rewrite map_id.
+    + rewrite -(map_id l'). now eapply Forall2_map.
+  Qed.
+
+  Definition lookup_constructor_args Σ ind : option (list nat) 
+    := match lookup_inductive Σ ind with
+    | Some (_, idecl) => Some (map cstr_nargs (ind_ctors idecl))
+   | None => None
+    end.
+
+Inductive Forall2i {A B : Type} (R : nat -> A -> B -> Prop) (n : nat)
+  : list A -> list B -> Prop :=
+| Forall2i_nil : Forall2i R n [] []
+| Forall2i_cons :
+    forall x y l r,
+      R n x y ->
+      Forall2i R (S n) l r ->
+      Forall2i R n (x :: l) (y :: r).
+Arguments Forall2i_nil {_ _ _ _}.
+Arguments Forall2i_cons {_ _ _ _ _ _ _ _}.
+
+Derive Signature NoConfusionHom for All2i.
+
+Lemma Forall2_Forall_mix {A B} {P : B -> Prop} {Q : A -> B -> Prop}
+   {l : list A} {l' : list B} :
+  Forall2 (fun x y => (P y -> Q x y)) l l' -> Forall P l' -> Forall2 Q l l'.
+Proof.
+  induction 1; simpl; intros; constructor; inversion H1; eauto.
+Qed.
+
+  Lemma Forall2_and_inv {A B : Type} (R R' : A -> B -> Prop) (l : list A) (l' : list B) :
+    Forall2 (fun (x : A) (y : B) => R x y /\ R' x y) l l'
+    -> Forall2 R l l' /\ Forall2 R' l l'.
+  Proof.
+    induction 1; split; eauto; econstructor; destruct H; now destruct IHForall2.
+  Qed.
+
+  Section Pure.
+
+  Variable Σ : list Ident.t.
+
+  Fixpoint isPure (t : t) :=
+    match t with
+    | Mvar x => true
+    | Mlambda (ids, x) => isPure x
+    | Mapply (x, args) => isPure x && forallb isPure args
+    | Mlet (binds, x) => forallb isPure_binding binds && isPure x
+    | Mnum x => true
+    | Mstring x => false (* strings are interpreted using vectors *)
+    | Mglobal id => true
+    | Mswitch (x, sels) => isPure x && forallb (fun '(_, x) => isPure x) sels
+    | Mnumop1 (op, num, x) => isPure x
+    | Mnumop2 (op, num, x1, x2) => isPure x1 && isPure x2
+    | Mconvert (from, to, x) => isPure x
+    | Mblock (tag, xs) => forallb isPure xs
+    | Mfield (i, x) => isPure x
+    | _ => false
+    end
+  with isPure_binding (b : binding) :=
+         match b with
+         | Unnamed x => isPure x
+         | Named (id, x) => isPure x
+         | Recursive recs => forallb (fun '(id,x) => isPure x) recs
+         end.
+
+  Definition isPure_rec_value `{Heap} (v : rec_value) :=
+    match v with 
+    | RFunc (_ , t) => is_true (isPure t)
+    | Bad_recursive_value => True
+    | _ => False
+    end. 
+
+  Fixpoint isPure_value `{Heap} (v : value) {struct v} :=
+    match v with
+    | Block (_,vs) => Forall (fun p => p) (map isPure_value vs)
+    | Func (locals,_,t) => (forall s, isPure_value (locals s)) /\ is_true (isPure t)    
+    | RClos (locals,self,mfix,t) => (forall s, isPure_value (locals s)) /\ Forall isPure_rec_value mfix
+    | value_Int _ => True
+    | Float _ => True
+    | fail _ => True
+    | _ => False
+    end.
+
+End Pure.
+
+From Malfunction Require Import CompileCorrect Pipeline.
+
+Lemma isPure_add_self `{Heap} locals mfix self s :
+  (forall s : Ident.t, isPure_value (locals s)) ->
+  Forall isPure_rec_value mfix ->
+  isPure_value (add_self self mfix locals s).
+Proof.
+  intros Hlocals Hmfix. unfold add_self, add_recs, List.mapi.
+  generalize 0 as i. generalize self at 1. 
+  induction self; cbn; eauto.
+  unfold Ident.Map.add. destruct (Ident.eqb s a); cbn; eauto.
+Qed.
+
+Lemma isPure_heap `{Heap} `{WcbvFlags} locals h h' t v :
+  is_true (isPure t) ->
+  (forall s, isPure_value (locals s)) -> 
+  eval [] locals h t h' v -> isPure_value v /\ h = h'.
+Proof.
+  intros Hpure Hlocals. induction 1; try solve [inversion Hpure]; cbn in Hpure;
+  repeat rewrite MCProd.andb_and in Hpure; try solve [cbn; repeat split; eauto]; eauto. 
+  - cbn in *. destruct Hpure as [? [? ?]].
+    try (destruct IHeval1; eauto);
+     try (destruct IHeval2; eauto); try (destruct IHeval3; eauto); try now eauto.
+    destruct H4. intros s. unfold Ident.Map.add. destruct (Ident.eqb s x); eauto.
+  - destruct Hpure as [? [? ?]].
+    try (destruct IHeval1; eauto);
+     try (destruct IHeval2; eauto); try (destruct IHeval3; eauto); try now eauto.
+    destruct H5. pose proof (proj1 (Forall_nth _ _) H9 n Bad_recursive_value). rewrite H1 in H10.
+    eapply H10. case_eq (Nat.ltb n #|mfix|); try rewrite Nat.ltb_lt; eauto.
+    rewrite Nat.ltb_ge. intro neq.  rewrite nth_overflow in H1; eauto. inversion H1.  
+    destruct H5. intros s. unfold Ident.Map.add. destruct (Ident.eqb s y); eauto.
+    eapply isPure_add_self; eauto. 
+  - cbn in *. destruct Hpure as [? [? ?]]; try (destruct IHeval1; eauto); now eauto.
+  - destruct Hpure as [? [? [? ?]]]. repeat rewrite MCProd.andb_and in IHeval.
+    destruct IHeval ; eauto.
+  - cbn in *. destruct Hpure as [[? ?] ?]; try (destruct IHeval1; eauto); try (destruct IHeval2; eauto); now eauto.  
+  - cbn in *. destruct Hpure as [[? ?] ?]; try (destruct IHeval1; eauto); try (destruct IHeval2; eauto); try now eauto.
+    intros s. unfold Ident.Map.add. destruct (Ident.eqb s x); eauto.
+  - cbn in *. destruct Hpure as [[? ?] ?]; try (destruct IHeval; eauto); try now eauto.
+    intros s. rewrite H1. eapply isPure_add_self; eauto. unfold rfunc, RFunc_build.
+    eapply forallb_Forall in H3. clear -H3. induction recs; eauto; cbn. destruct a; cbn in *. inversion H3; subst.
+    econstructor; eauto. destruct t0; cbn; eauto. destruct p. cbn in H2. destruct l; cbn ; eauto.
+    destruct l; cbn ; eauto.
+  - cbn in *. destruct Hpure as [? ?]; try (destruct IHeval1; eauto); try (destruct IHeval2; eauto); try now eauto.
+    induction cases; cbn in *. inversion H1. repeat rewrite MCProd.andb_and in H3. destruct H3.   
+    destruct a. destruct (existsb _ _); [inversion H1; subst; eauto|]. now eapply IHcases.
+  - cbn in *. clear H1 H2. induction H3; [now eauto|]. repeat rewrite MCProd.andb_and in Hpure.
+    destruct Hpure. destruct IHForall2_acc; eauto. destruct H1; eauto. cbn; split; now eauto.
+  - cbn in *. destruct IHeval; eauto. split; eauto. eapply Forall_nth; eauto. now eapply Forall_map_inv in H4.
+  - cbn in *. now eauto.
+  - cbn in *. inversion H1.
+  - cbn in *. destruct IHeval; eauto.
+  - cbn. destruct Hpure. destruct IHeval1; eauto. destruct IHeval2; eauto. now destruct op.
+  - cbn; now eauto.   
+  - cbn; destruct Hpure. destruct IHeval1; eauto. destruct IHeval2; now eauto.
+  - cbn; destruct Hpure. destruct IHeval1; eauto. destruct IHeval2; now eauto.
+  - cbn; destruct IHeval; eauto. 
+  - cbn. destruct IHeval; eauto.
+  - cbn. destruct IHeval; eauto.
+Qed.            
+
+Lemma isPure_heap_irr `{Heap} `{WcbvFlags} h h' locals t v :
+  is_true (isPure t) ->
+  (forall s, isPure_value (locals s)) -> 
+  eval [] locals h t h' v -> forall h'', eval [] locals h'' t h'' v.
+Proof.
+  intros Hpure Hlocals. induction 1; try solve [inversion Hpure]; cbn in Hpure;
+  repeat rewrite MCProd.andb_and in Hpure; try solve [cbn; destruct Hpure; econstructor; eauto]; 
+  try solve [cbn; econstructor; eauto].
+  - intro. destruct Hpure as [? [? ?]]. econstructor 3; eauto.
+    eapply isPure_heap in H1_, H1_0; eauto. destruct H1_ as [[Hlocals' He] _].  
+    eapply IHeval3; eauto. intros s. unfold Ident.Map.add. destruct (Ident.eqb s x); now eauto.
+  - intro. destruct Hpure as [? [? ?]]. econstructor 4; eauto.
+    eapply isPure_heap in H1_, H1_0; eauto. destruct H1_ as [[Hlocals' He] _].
+    pose proof (proj1 (Forall_nth _ _) He n Bad_recursive_value).
+    rewrite H1 in H5. cbn in H5. eapply IHeval3.
+    case_eq (Nat.ltb n #|mfix|); try rewrite Nat.ltb_lt; eauto.
+    rewrite Nat.ltb_ge. intro neq. rewrite nth_overflow in H1; eauto. inversion H1.  
+    destruct H1_0. intros s. unfold Ident.Map.add. destruct (Ident.eqb s y); eauto.
+    eapply isPure_add_self; eauto. 
+  - intro. destruct Hpure as [? [? ?]]. econstructor 6; eauto.
+    eapply IHeval; eauto. cbn. now repeat rewrite MCProd.andb_and.
+  - intro. destruct Hpure as [[? ?] ?]. econstructor; eauto. eapply IHeval2; eauto. 
+    cbn. now repeat rewrite MCProd.andb_and.
+  - intro. destruct Hpure as [[? ?] ?]. econstructor; eauto. eapply IHeval2; eauto. 
+    cbn. now repeat rewrite MCProd.andb_and. 
+    intros s. unfold Ident.Map.add. destruct (Ident.eqb s x); eauto. eapply isPure_heap in H1_; now eauto. 
+  - intro. destruct Hpure as [[? ?] ?]. econstructor; eauto. rewrite H1 in IHeval. eapply IHeval; eauto; cbn.
+    now repeat rewrite MCProd.andb_and. intro s. eapply isPure_add_self; eauto.
+    unfold rfunc, RFunc_build.
+    eapply forallb_Forall in H3. clear -H3. induction recs; eauto; cbn. destruct a; cbn in *. inversion H3; subst.
+    econstructor; eauto. destruct t0; cbn; eauto. destruct p. cbn in H2. destruct l; cbn ; eauto.
+    destruct l; cbn ; eauto. 
+  - destruct Hpure. econstructor; eauto. eapply IHeval2; eauto.   
+    induction cases; cbn in *. inversion H1. repeat rewrite MCProd.andb_and in H3. destruct H3.   
+    destruct a. destruct (existsb _ _); [inversion H1; subst; eauto|]. now eapply IHcases.
+  - econstructor; eauto. clear H1 H2. induction H3; [econstructor; eauto|].
+    cbn in Hpure. rewrite MCProd.andb_and in Hpure. destruct Hpure. econstructor; eauto.
+Qed.
